ed25519: prove point_inv for [2^64]G, [2^128]G and [2^192]G

code/ed25519/Hacl.Ed25519.PrecompTable.fst
@@ -11,6 +11,7 @@ open Hacl.Bignum25519
 module F51 = Hacl.Impl.Ed25519.Field51
 
 module LSeq = Lib.Sequence
+module LM = Lib.NatMod
 module LE = Lib.Exponentiation
 module SE = Spec.Exponentiation
 module SPT = Hacl.Spec.PrecompBaseTable
@@ -31,6 +32,39 @@ let lemma_refl x =
   SPTE.ext_point_to_list_lemma x
 
 //-----------------
+
+val lemma_is_on_curve: x:SC.elem -> y:SC.elem ->
+  Lemma (Spec.Curve25519.(y *% y -% x *% x) == (y * y - x * x) % SC.prime /\
+  Spec.Curve25519.(1 +% S.d *% (x *% x) *% (y *% y)) == (1 + S.d * (x * x) * (y * y)) % SC.prime)
+
+let lemma_is_on_curve x y =
+  let open Spec.Curve25519 in
+  let open Spec.Ed25519 in
+  calc (==) {
+    y *% y -% x *% x;
+    (==) { }
+    ((y * y) % prime - (x * x) % prime) % prime;
+    (==) { Math.Lemmas.lemma_mod_plus_distr_l (y * y) (- (x * x) % prime) prime }
+    (y * y - (x * x) % prime) % prime;
+    (==) { Math.Lemmas.lemma_mod_sub_distr (y * y) (x * x) prime }
+    (y * y - x * x) % prime;
+    };
+
+  calc (==) {
+    1 +% S.d *% (x *% x) *% (y *% y);
+    (==) { }
+    (1 + (S.d * (x * x % prime) % prime) * (y * y % prime) % prime) % prime;
+    (==) { Math.Lemmas.lemma_mod_mul_distr_r S.d (x * x) prime }
+    (1 + (S.d * (x * x) % prime) * (y * y % prime) % prime) % prime;
+    (==) { Math.Lemmas.lemma_mod_mul_distr_l (S.d * (x * x)) (y * y % prime) prime }
+    (1 + (S.d * (x * x)) * (y * y % prime) % prime) % prime;
+    (==) { Math.Lemmas.lemma_mod_mul_distr_r (S.d * (x * x)) (y * y) prime }
+    (1 + (S.d * (x * x)) * (y * y) % prime) % prime;
+    (==) { Math.Lemmas.lemma_mod_plus_distr_r 1 ((S.d * (x * x)) * (y * y)) prime }
+    (1 + (S.d * (x * x)) * (y * y)) % prime;
+    }
+
+//--------------
 
 let ext_g_pow2_64 : S.ext_point =
   [@inline_let]
@@ -57,10 +91,45 @@ let lemma_ext_g_pow2_64_eval () =
   let rT : SC.elem = 0x75e4cec7f1c8417c2268c6cff4e4f9d94dd599649b949e8e19cf23c11f401586 in
   assert_norm (qX == rX /\ qY == rY /\ qZ == rZ /\ qT == rT)
 
+
+val ext_g_pow2_64_zinv: unit -> Lemma (let (rX, rY, rZ, rT) = ext_g_pow2_64 in
+  SC.finv rZ = 0x32435c2ae3ace33871119d9346f332af7d025740cdca88b087ec408e4b7b1c76)
+
+let ext_g_pow2_64_zinv () =
+  let rZ = 0x424da3d215aef3b7967274a7d81d8d30e7a51756922ebd07058c9d04ac8405e0 in
+  let rZ_comp = normalize_term (LM.pow_mod_ #SC.prime rZ (SC.prime - 2)) in
+  normalize_term_spec (LM.pow_mod_ #SC.prime rZ (SC.prime - 2));
+  assert_norm (rZ_comp ==
+    0x32435c2ae3ace33871119d9346f332af7d025740cdca88b087ec408e4b7b1c76);
+
+  let (_, _, qZ, _) = ext_g_pow2_64 in
+  assert (qZ == rZ);
+  LM.pow_mod_def #SC.prime rZ (SC.prime - 2)
+
+
 val lemma_ext_g_pow2_64_point_inv: unit -> Lemma (S.point_inv ext_g_pow2_64)
 let lemma_ext_g_pow2_64_point_inv () =
-  assume (S.is_on_curve (S.to_aff_point ext_g_pow2_64));
-  assume (S.is_ext ext_g_pow2_64)
+  let open Spec.Curve25519 in
+  let open Spec.Ed25519 in
+  let rX : SC.elem = 0x5a8a5a58bef144743ef0a14ef1bad8b169be613a4f82d2c418c00c5507edf10d in
+  let rY : SC.elem = 0x1ad2dd576455f6786b43640245cf64fae933ffc7ecabc74b63ce54790e453f73 in
+  let rZ : SC.elem = 0x424da3d215aef3b7967274a7d81d8d30e7a51756922ebd07058c9d04ac8405e0 in
+  let rT : SC.elem = 0x75e4cec7f1c8417c2268c6cff4e4f9d94dd599649b949e8e19cf23c11f401586 in
+  let zinv : SC.elem = 0x32435c2ae3ace33871119d9346f332af7d025740cdca88b087ec408e4b7b1c76 in
+  ext_g_pow2_64_zinv ();
+  let (x, y) = (rX *% zinv, rY *% zinv) in
+  assert (x = 0x6222bd88bf2df9d5d44b60cfb4a08a960078db7ed51a35eb3e0b6b8ff4eda202);
+  assert (y = 0x325bb42ea4ed025dd6bdaed261b7c4f5410b608ba902b068f1efa5782e45313);
+  lemma_is_on_curve x y;
+  assert ((y * y - x * x) % SC.prime =
+    0x44b4161cc56730b0c4ddd3ee61af107f6ec87d11e0da287cb1dc61a07d10842a);
+  assert ((1 + d * (x * x) * (y * y)) % SC.prime =
+    0x44b4161cc56730b0c4ddd3ee61af107f6ec87d11e0da287cb1dc61a07d10842a);
+  assert (S.is_on_curve (x, y));
+  assert (rX *% rY *% zinv =
+    0x75e4cec7f1c8417c2268c6cff4e4f9d94dd599649b949e8e19cf23c11f401586);
+  assert (S.is_ext ext_g_pow2_64)
+
 
 let ext_g_pow2_64_c : S.ext_point_c =
   lemma_ext_g_pow2_64_point_inv ();
@@ -92,10 +161,45 @@ let lemma_ext_g_pow2_128_eval () =
   let rT : SC.elem = 0x3dc4d80a0c809ab67253c9cae46b0a2fdbfca8ca0f515475b21d1e95fb8d9add in
   assert_norm (qX == rX /\ qY == rY /\ qZ == rZ /\ qT == rT)
 
+
+val ext_g_pow2_128_zinv: unit -> Lemma (let (rX, rY, rZ, rT) = ext_g_pow2_128 in
+  SC.finv rZ = 0xa908d480f92385648adf4303f41d185348ebd63cea140b01be3c2e3b13b378)
+
+let ext_g_pow2_128_zinv () =
+  let rZ = 0x78d98ebac33bd94604a2ce24527eb73c2cba4d3b1e5f55b8444bb5e513a54540 in
+  let rZ_comp = normalize_term (LM.pow_mod_ #SC.prime rZ (SC.prime - 2)) in
+  normalize_term_spec (LM.pow_mod_ #SC.prime rZ (SC.prime - 2));
+  assert_norm (rZ_comp ==
+    0xa908d480f92385648adf4303f41d185348ebd63cea140b01be3c2e3b13b378);
+
+  let (_, _, qZ, _) = ext_g_pow2_128 in
+  assert (qZ == rZ);
+  LM.pow_mod_def #SC.prime rZ (SC.prime - 2)
+
+
 val lemma_ext_g_pow2_128_point_inv: unit -> Lemma (S.point_inv ext_g_pow2_128)
 let lemma_ext_g_pow2_128_point_inv () =
-  assume (S.is_on_curve (S.to_aff_point ext_g_pow2_128));
-  assume (S.is_ext ext_g_pow2_128)
+  let open Spec.Curve25519 in
+  let open Spec.Ed25519 in
+  let rX : SC.elem = 0x38569441a1f5cd408a120bf398c05f4d98921fc59796c50c2af9fb1690e8727e in
+  let rY : SC.elem = 0x0a97dfad58fa26197529d9296502368db1c0513ba4c45512f239db96f78d2e7c in
+  let rZ : SC.elem = 0x78d98ebac33bd94604a2ce24527eb73c2cba4d3b1e5f55b8444bb5e513a54540 in
+  let rT : SC.elem = 0x3dc4d80a0c809ab67253c9cae46b0a2fdbfca8ca0f515475b21d1e95fb8d9add in
+  let zinv : SC.elem = 0xa908d480f92385648adf4303f41d185348ebd63cea140b01be3c2e3b13b378 in
+  ext_g_pow2_128_zinv ();
+  let (x, y) = (rX *% zinv, rY *% zinv) in
+  assert (x = 0x4c27afff3c45f32c952d3984e14e29a098e685c9c2e723e5fc8047ae60b7e824);
+  assert (y = 0x5f2c99e6526dc87d95f11eb626c29c3a90d0be1e51a4c49e5bbabd114bf5a66b);
+  lemma_is_on_curve x y;
+  assert ((y * y - x * x) % SC.prime =
+    0x1a6a9dfe3e20bc6d73e5c689df4c1b7d21d6a7d878feb81680f0e5cb6e31ea55);
+  assert ((1 + d * (x * x) * (y * y)) % SC.prime =
+    0x1a6a9dfe3e20bc6d73e5c689df4c1b7d21d6a7d878feb81680f0e5cb6e31ea55);
+  assert (S.is_on_curve (x, y));
+  assert (rX *% rY *% zinv =
+    0x3dc4d80a0c809ab67253c9cae46b0a2fdbfca8ca0f515475b21d1e95fb8d9add);
+  assert (S.is_ext ext_g_pow2_128)
+
 
 let ext_g_pow2_128_c : S.ext_point_c =
   lemma_ext_g_pow2_128_point_inv ();
@@ -127,10 +231,45 @@ let lemma_ext_g_pow2_192_eval () =
   let rT : SC.elem = 0x4ba921103721bfbb5070816bf7abc2fcb5fb2e653f32d7188e21c4170e2d4e01 in
   assert_norm (qX == rX /\ qY == rY /\ qZ == rZ /\ qT == rT)
 
+
+val ext_g_pow2_192_zinv: unit -> Lemma (let (rX, rY, rZ, rT) = ext_g_pow2_192 in
+  SC.finv rZ = 0x2972deff9b37f94926b9a4d6b37f37d190689259040e63ed0da418e98c52b9d4)
+
+let ext_g_pow2_192_zinv () =
+  let rZ = 0x7d0300628a3869589b68ed3d9c968775e69a9e2a7c7913184c5af18b60a3effb in
+  let rZ_comp = normalize_term (LM.pow_mod_ #SC.prime rZ (SC.prime - 2)) in
+  normalize_term_spec (LM.pow_mod_ #SC.prime rZ (SC.prime - 2));
+  assert_norm (rZ_comp ==
+    0x2972deff9b37f94926b9a4d6b37f37d190689259040e63ed0da418e98c52b9d4);
+
+  let (_, _, qZ, _) = ext_g_pow2_192 in
+  assert (qZ == rZ);
+  LM.pow_mod_def #SC.prime rZ (SC.prime - 2)
+
+
 val lemma_ext_g_pow2_192_point_inv: unit -> Lemma (S.point_inv ext_g_pow2_192)
 let lemma_ext_g_pow2_192_point_inv () =
-  assume (S.is_on_curve (S.to_aff_point ext_g_pow2_192));
-  assume (S.is_ext ext_g_pow2_192)
+  let open Spec.Curve25519 in
+  let open Spec.Ed25519 in
+  let rX : SC.elem = 0x59a2726d1a927e56005542ff7c0dded153e9146340a7ba261e0403afbd77ba7d in
+  let rY : SC.elem = 0x09344b8ad2982520f18314ea851cebe018a16987ad52191e466d5c1d19f5096d in
+  let rZ : SC.elem = 0x7d0300628a3869589b68ed3d9c968775e69a9e2a7c7913184c5af18b60a3effb in
+  let rT : SC.elem = 0x4ba921103721bfbb5070816bf7abc2fcb5fb2e653f32d7188e21c4170e2d4e01 in
+  let zinv : SC.elem = 0x2972deff9b37f94926b9a4d6b37f37d190689259040e63ed0da418e98c52b9d4 in
+  ext_g_pow2_192_zinv ();
+  let (x, y) = (rX *% zinv, rY *% zinv) in
+  assert (x = 0x1bc7af1e38185e7c2d8d04371c7e177d7a9ddee1b81d7d26db7ad644c7dad28d);
+  assert (y = 0x61d909d855661f2f7a5eef87795dc0491d027e12631b270fcaf2f65900314833);
+  lemma_is_on_curve x y;
+  assert ((y * y - x * x) % SC.prime =
+    0x17b3d90b42ff679b6cc94130e36b67e6a1fe8292c22f4e6f1cdff4a37fecafd8);
+  assert ((1 + d * (x * x) * (y * y)) % SC.prime =
+    0x17b3d90b42ff679b6cc94130e36b67e6a1fe8292c22f4e6f1cdff4a37fecafd8);
+  assert (S.is_on_curve (x, y));
+  assert (rX *% rY *% zinv =
+    0x4ba921103721bfbb5070816bf7abc2fcb5fb2e653f32d7188e21c4170e2d4e01);
+  assert (S.is_ext ext_g_pow2_192)
+
 
 let ext_g_pow2_192_c : S.ext_point_c =
   lemma_ext_g_pow2_192_point_inv ();
